Prove wp_volumeClaimTemplatesByName

src/proof/controllers/statefulset/progress.v
@@ -492,6 +492,203 @@ Proof.
     by apply Hpod_meta_Hdeepown_deletiontimestamp_none.
 Qed.
 
+Definition claim_templates_map_insert m claim_template : gmap go_string v1.PersistentVolumeClaim.t :=
+  <[claim_template.(v1.PersistentVolumeClaim.ObjectMeta').(v1.ObjectMeta.Name') := claim_template]> m.
+
+Definition claim_templates_map_of_list claim_templates : gmap go_string v1.PersistentVolumeClaim.t :=
+  fold_left claim_templates_map_insert claim_templates ∅.
+
+Lemma claim_templates_map_of_list_snoc claim_templates claim_template :
+  claim_templates_map_of_list (claim_templates ++ [claim_template]) =
+  claim_templates_map_insert (claim_templates_map_of_list claim_templates) claim_template.
+Proof.
+  unfold claim_templates_map_of_list.
+  by rewrite fold_left_app.
+Qed.
+
+Lemma claim_templates_map_of_list_values claim_templates :
+  map_Forall (λ name claim_template,
+    claim_template ∈ claim_templates ∧
+    claim_template.(v1.PersistentVolumeClaim.ObjectMeta').(v1.ObjectMeta.Name') = name)
+    (claim_templates_map_of_list claim_templates).
+Proof.
+  induction claim_templates using rev_ind.
+  - rewrite /claim_templates_map_of_list /=.
+    apply map_Forall_empty.
+  - rewrite claim_templates_map_of_list_snoc.
+    rewrite map_Forall_lookup.
+    intros name claim_template Hlookup.
+    unfold claim_templates_map_insert in Hlookup.
+    apply lookup_insert_Some in Hlookup as [[<- <-]|[Hname_ne Hlookup]].
+    + split; [apply elem_of_app; right; by left|done].
+    + rewrite map_Forall_lookup in IHclaim_templates.
+      specialize (IHclaim_templates _ _ Hlookup) as [Hin Hname].
+      split; [apply elem_of_app; by left|done].
+Qed.
+
+Lemma claim_templates_map_of_list_names claim_templates :
+  Forall (λ claim_template,
+    is_Some (claim_templates_map_of_list claim_templates !!
+      claim_template.(v1.PersistentVolumeClaim.ObjectMeta').(v1.ObjectMeta.Name')))
+    claim_templates.
+Proof.
+  induction claim_templates using rev_ind.
+  - done.
+  - apply Forall_forall. intros claim_template Hin.
+    rewrite claim_templates_map_of_list_snoc /claim_templates_map_insert.
+    apply in_app_or in Hin.
+    destruct Hin as [Hin|Hin].
+    + rewrite Forall_forall in IHclaim_templates.
+      destruct (IHclaim_templates claim_template Hin) as [mapped Hlookup].
+      destruct (decide (
+        x.(v1.PersistentVolumeClaim.ObjectMeta').(v1.ObjectMeta.Name') =
+        claim_template.(v1.PersistentVolumeClaim.ObjectMeta').(v1.ObjectMeta.Name'))) as
+        [Heq|Hne].
+      * exists x. by rewrite Heq lookup_insert_eq.
+      * exists mapped. by rewrite lookup_insert_ne.
+    + destruct Hin as [<-|[]].
+      exists x. by rewrite lookup_insert_eq.
+Qed.
+
+(* The returned map contains physical PVC template values copied from the
+   StatefulSet's physical VolumeClaimTemplates slice.  Keeping the StatefulSet
+   deep ownership split in the postcondition exposes that physical slice and
+   lets callers relate map entries back to the concrete templates without
+   immediately hiding the fields behind StatefulSetV.deepown_l again. *)
+Lemma wp_volumeClaimTemplatesByName set_l (set : StatefulSetV.t) dq :
+  {{{ StatefulSetV.deepown_l set_l set dq }}}
+    @! statefulset.volumeClaimTemplatesByName #set_l
+  {{{ (set_phy : v1.StatefulSet.t) claim_templates_map claim_templates_list
+      (claim_templates_phy : gmap go_string v1.PersistentVolumeClaim.t),
+      RET #claim_templates_map;
+      set_l ↦{dq} set_phy ∗
+      "%Hdeepown_typemeta" ∷ ⌜ set_phy.(v1.StatefulSet.TypeMeta') = set.(StatefulSetV.TypeMeta') ⌝ ∗
+      "Hdeepown_objectmeta" ∷
+        ObjectMetaV.deepown set_phy.(v1.StatefulSet.ObjectMeta') set.(StatefulSetV.ObjectMeta') dq ∗
+      "%Hdeepown_replicas_none" ∷
+        ⌜ set_phy.(v1.StatefulSet.Spec').(v1.StatefulSetSpec.Replicas') = null ↔
+          set.(StatefulSetV.Spec').(StatefulSetSpecV.Replicas') = None ⌝ ∗
+      "Hdeepown_replicas_some" ∷
+        (match set.(StatefulSetV.Spec').(StatefulSetSpecV.Replicas') with
+        | Some i =>
+            ∃ replicas,
+              set_phy.(v1.StatefulSet.Spec').(v1.StatefulSetSpec.Replicas') ↦{dq} replicas ∗
+              ⌜ replicas = i ⌝
+        | None => True%I
+        end) ∗
+      "Hdeepown_template" ∷ PodTemplateSpecV.deepown set_phy.(v1.StatefulSet.Spec').(v1.StatefulSetSpec.Template')
+          set.(StatefulSetV.Spec').(StatefulSetSpecV.Template') dq ∗
+      "Hdeepown_volumeclaimtemplates" ∷ deepown_list
+        set_phy.(v1.StatefulSet.Spec').(v1.StatefulSetSpec.VolumeClaimTemplates') claim_templates_list
+          set.(StatefulSetV.Spec').(StatefulSetSpecV.VolumeClaimTemplates')
+          (λ claim_template_phy pure_claim_template,
+            PersistentVolumeClaimV.deepown claim_template_phy pure_claim_template dq) ∗
+      "%Hclaim_templates_map_values" ∷
+        ⌜ map_Forall (λ name claim_template_phy,
+            claim_template_phy ∈ claim_templates_list ∧
+            claim_template_phy.(v1.PersistentVolumeClaim.ObjectMeta').(v1.ObjectMeta.Name') = name
+          ) claim_templates_phy ⌝ ∗
+      "%Hclaim_templates_list_names" ∷
+        ⌜ Forall (λ claim_template_phy,
+            is_Some (claim_templates_phy !!
+              claim_template_phy.(v1.PersistentVolumeClaim.ObjectMeta').(v1.ObjectMeta.Name'))
+          ) claim_templates_list ⌝ ∗
+      "%Hdeepown_servicename" ∷
+        ⌜ set_phy.(v1.StatefulSet.Spec').(v1.StatefulSetSpec.ServiceName') =
+          set.(StatefulSetV.Spec').(StatefulSetSpecV.ServiceName') ⌝ ∗
+      "Hdeepown_status" ∷ StatefulSetStatusV.deepown set_phy.(v1.StatefulSet.Status') set.(StatefulSetV.Status') dq ∗
+      "Hclaim_templates_map" ∷ claim_templates_map ↦$ claim_templates_phy
+  }}}.
+Proof.
+  wp_start as "Hset".
+  iDestruct "Hset" as (set_phy) "[Hset_ptr Hset_deepown]".
+  iNamed "Hset_deepown".
+  iNamed "Hdeepown_spec".
+  iDestruct "Hdeepown_volumeclaimtemplates" as (claim_templates_list)
+    "Hdeepown_volumeclaimtemplates".
+  rewrite /deepown_list.
+  iDestruct "Hdeepown_volumeclaimtemplates" as
+    "[Hclaim_templates_slice Hclaim_templates_deepown]".
+  wp_auto.
+  wp_apply wp_map_make2 as "%claim_templates_map Hclaim_templates_map".
+  iDestruct (own_slice_len with "Hclaim_templates_slice") as
+    %(Hclaim_templates_len1 & Hclaim_templates_len2).
+  iDestruct (own_slice_wf with "Hclaim_templates_slice") as
+    %Hclaim_templates_cap.
+  iDestruct (big_sepL2_length with "Hclaim_templates_deepown") as
+    %Hclaim_templates_deepown_len.
+  set I := (∃ (i : w64) (claim_template_value : v1.PersistentVolumeClaim.t)
+      (claim_templates_map_l : map.t),
+    "Hi_ptr" ∷ i_ptr ↦ i ∗
+    "Hclaim_templates_slice" ∷
+      set_phy.(v1.StatefulSet.Spec').(v1.StatefulSetSpec.VolumeClaimTemplates') ↦*
+        claim_templates_list ∗
+    "HclaimTemplate_ptr" ∷ claimTemplate_ptr ↦ claim_template_value ∗
+    "HclaimTemplates_ptr" ∷ claimTemplates_ptr ↦ claim_templates_map_l ∗
+    "Hclaim_templates_map" ∷ claim_templates_map_l ↦$
+      claim_templates_map_of_list (take (sint.nat i) claim_templates_list) ∗
+    "%Hi" ∷ ⌜ 0 ≤ sint.Z i ≤ sint.Z
+      (slice.len set_phy.(v1.StatefulSet.Spec').(v1.StatefulSetSpec.VolumeClaimTemplates')) ⌝
+  )%I.
+  iAssert I with "[i Hclaim_templates_slice claimTemplate claimTemplates
+      Hclaim_templates_map]" as
+    "Hloop_inv".
+  { iExists (W64 0), (zero_val v1.PersistentVolumeClaim.t), claim_templates_map.
+    rewrite take_0 /claim_templates_map_of_list /=.
+    iFrame.
+    iPureIntro. word. }
+  wp_for "Hloop_inv". wp_if_destruct.
+  - destruct (decide (0 ≤ sint.Z i <
+      sint.Z (slice.len set_phy.(v1.StatefulSet.Spec').(v1.StatefulSetSpec.VolumeClaimTemplates'))))
+      as [_|Hbounds]; last word.
+    assert (∃ this_claim_template,
+      claim_templates_list !! sint.nat i = Some this_claim_template) as
+      [this_claim_template Hthis_claim_template_lookup].
+    { apply lookup_lt_is_Some_2. rewrite Hclaim_templates_len1. word. }
+    wp_apply (wp_load_slice_index with "[$Hclaim_templates_slice]"); [word| |].
+    { iPureIntro. exact Hthis_claim_template_lookup. }
+    iIntros "Hclaim_templates_slice".
+    wp_auto.
+    wp_apply (wp_map_insert go.string with "[$Hclaim_templates_map]").
+    iIntros "Hclaim_templates_map".
+    wp_auto.
+    iApply wp_for_post_do.
+    wp_auto.
+    iFrame "HΦ".
+    iFrame "Hset_ptr Hdeepown_objectmeta Hdeepown_replicas_some
+      Hdeepown_template Hclaim_templates_deepown Hdeepown_status".
+    iExists (word.add i (W64 1)), this_claim_template, claim_templates_map_l.
+    assert (claim_templates_map_of_list
+      (take (sint.nat (word.add i (W64 1))) claim_templates_list) =
+      claim_templates_map_insert
+        (claim_templates_map_of_list (take (sint.nat i) claim_templates_list))
+        this_claim_template) as Hmap_next.
+    { assert (sint.nat (word.add i (W64 1)) = S (sint.nat i)) as -> by word.
+      rewrite (take_S_r _ _ _ Hthis_claim_template_lookup).
+      apply claim_templates_map_of_list_snoc. }
+    rewrite Hmap_next.
+    iFrame.
+    iFrame "%".
+    iPureIntro. word.
+  - assert (take (sint.nat i) claim_templates_list = claim_templates_list) as Htake_all.
+    { assert (sint.nat i = length claim_templates_list) as Hi_len.
+      { rewrite Hclaim_templates_len1. word. }
+      rewrite Hi_len.
+      apply take_ge. lia. }
+    rewrite Htake_all.
+    iApply ("HΦ" $! set_phy claim_templates_map_l claim_templates_list
+      (claim_templates_map_of_list claim_templates_list)).
+    iFrame.
+    rewrite /deepown_list.
+    iFrame.
+    iFrame "%".
+    iSplit.
+    + iPureIntro. apply claim_templates_map_of_list_values.
+    + iPureIntro. apply claim_templates_map_of_list_names.
+Unshelve.
+  all: apply _.
+Qed.
+
 Lemma wp_filterPodsForStatefulSet set_l pods_sl
     (set : StatefulSetV.t) (ptrs : list loc) (pods : list PodV.t) dq_set dq_pods :
   {{{ "Hset" ∷ StatefulSetV.deepown_l set_l set dq_set ∗
